src/Bedrock/Field/Synthesis/New/UnsaturatedSolinas.v
@@ -117,10 +117,11 @@ Section UnsaturatedSolinas.
          (prime_bytes_upperbound_list s)).
   Local Instance field_representation : FieldRepresentation
     := field_representation
-         n (n_bytes s) weight
+         n (n_bytes s) weight (list (option ZRange.zrange))
          (UnsaturatedSolinasHeuristics.loose_bounds n s c)
          (UnsaturatedSolinasHeuristics.tight_bounds n s c)
-         (prime_bytes_bounds_value).
+         (prime_bytes_bounds_value)
+         list_Z_bounded_by (fun x => x) (fun x => x).
 
   Local Ltac specialize_correctness_hyp Hcorrect :=
     cbv [feval feval_bytes bounded_by bytes_in_bounds Field.loose_bounds
@@ -283,6 +284,14 @@ Section UnsaturatedSolinas.
     apply F.eq_of_Z_iff; rewrite ?F.to_Z_of_Z;
     cbv [M] in M_eq; rewrite ?M_eq; pull_Zmod.
 
+  Ltac loosen_bounds := lazymatch goal with
+  | |- forall _, list_Z_bounded_by ?thesebounds _ -> _ => simpl; intros; eapply relax_list_Z_bounded_by; [| eauto];
+    simpl; try apply tight_bounds_tighter_than; try apply loose_bounds_tighter_than
+  | _ => idtac
+  end.
+
+  Ltac bounds_length := simpl; intros; erewrite length_list_Z_bounded_by; eauto; try apply length_tight_bounds; try apply length_loose_bounds.
+
   Lemma mul_func_correct :
     valid_func (res mul_op _) ->
     forall functions,
@@ -294,7 +303,7 @@ Section UnsaturatedSolinas.
          _ _ _ _ _ ltac:(eassumption) _ (res_eq mul_op)
       as Hcorrect.
     eapply list_binop_correct with (res:=res mul_op);
-    handle_side_conditions; [ | | ].
+    handle_side_conditions; [ | | loosen_bounds | bounds_length ].
     { (* output *value* is correct *)
       intros. 
       specialize_correctness_hyp Hcorrect.
@@ -302,9 +311,6 @@ Section UnsaturatedSolinas.
       FtoZ; congruence. }
     { (* output *bounds* are correct *)
       intros. apply Hcorrect; auto. }
-    { cbv [bin_outbounds tight_bounds tight_upperbounds
-        prime_upperbound_list Partition.Partition.partition];
-        rewrite !map_length, seq_length; trivial. }
   Qed.
 
   Lemma square_func_correct :
@@ -318,16 +324,13 @@ Section UnsaturatedSolinas.
          _ _ _ _ _ ltac:(eassumption) _ (res_eq square_op)
       as Hcorrect.
     eapply list_unop_correct with (res:=res square_op);
-      handle_side_conditions; [ | | ].
+      handle_side_conditions; [ | | loosen_bounds| bounds_length ].
     { (* output *value* is correct *)
       intros. specialize_correctness_hyp Hcorrect.
       destruct Hcorrect. simpl_map_unsigned.
       rewrite F.pow_2_r. FtoZ; congruence. }
     { (* output *bounds* are correct *)
       intros. apply Hcorrect; auto. }
-    { cbv [un_outbounds tight_bounds tight_upperbounds
-        prime_upperbound_list Partition.Partition.partition];
-        rewrite !map_length, seq_length; trivial. }
   Qed.
 
   Lemma add_func_correct :
@@ -341,7 +344,7 @@ Section UnsaturatedSolinas.
          _ _ _ _ _ ltac:(eassumption) _ (res_eq add_op)
       as Hcorrect.
     eapply list_binop_correct with (res:=res add_op);
-    handle_side_conditions; [ | | ].
+    handle_side_conditions; [ | | loosen_bounds | bounds_length ].
     { (* output *value* is correct *)
       intros. 
       specialize_correctness_hyp Hcorrect.
@@ -349,10 +352,6 @@ Section UnsaturatedSolinas.
       FtoZ; congruence. }
     { (* output *bounds* are correct *)
       intros. apply Hcorrect; auto. }
-    { cbn. cbv [loose_bounds loose_upperbounds tight_upperbounds 
-        prime_upperbound_list Partition.Partition.partition  ].
-      rewrite !map_length,combine_length,!map_length,seq_length,length_balance.
-      eapply Nat.min_id. }
   Qed.
 
   Lemma sub_func_correct :
@@ -366,7 +365,7 @@ Section UnsaturatedSolinas.
          _ _ _ _ _ ltac:(eassumption) _ (res_eq sub_op)
       as Hcorrect.
     eapply list_binop_correct with (res:=res sub_op);
-    handle_side_conditions; [ | | ].
+    handle_side_conditions; [ | | loosen_bounds | bounds_length ].
     { (* output *value* is correct *)
       intros. 
       specialize_correctness_hyp Hcorrect.
@@ -374,10 +373,6 @@ Section UnsaturatedSolinas.
       rewrite <-F.of_Z_sub. FtoZ. congruence. }
     { (* output *bounds* are correct *)
       intros. apply Hcorrect; auto. }
-    { cbn. cbv [loose_bounds loose_upperbounds tight_upperbounds 
-        prime_upperbound_list Partition.Partition.partition  ].
-      rewrite !map_length,combine_length,!map_length,seq_length,length_balance.
-      eapply Nat.min_id. }
   Qed.
 
   Lemma opp_func_correct :
@@ -391,17 +386,13 @@ Section UnsaturatedSolinas.
       as Hcorrect.
 
     eapply list_unop_correct with (res:=res opp_op);
-      handle_side_conditions; [ | | ].
+      handle_side_conditions; [ | | loosen_bounds | bounds_length ].
     { (* output *value* is correct *)
       intros. specialize_correctness_hyp Hcorrect.
       destruct Hcorrect. simpl_map_unsigned.
       FtoZ. rewrite Z.sub_0_l; congruence. }
     { (* output *bounds* are correct *)
       intros. apply Hcorrect; auto. }
-    { cbn. cbv [loose_bounds loose_upperbounds tight_upperbounds 
-        prime_upperbound_list Partition.Partition.partition  ].
-      rewrite !map_length,combine_length,!map_length,seq_length,length_balance.
-      eapply Nat.min_id. }
   Qed.
 
   Lemma scmula24_func_correct :
@@ -417,16 +408,13 @@ Section UnsaturatedSolinas.
       as Hcorrect.
 
     eapply list_unop_correct with (res:=res scmula24_op);
-      handle_side_conditions; [ | | ].
+      handle_side_conditions; [ | | loosen_bounds | bounds_length ].
     { (* output *value* is correct *)
       intros. specialize_correctness_hyp Hcorrect.
       destruct Hcorrect. simpl_map_unsigned.
       FtoZ. congruence. }
     { (* output *bounds* are correct *)
       intros. apply Hcorrect; auto. }
-    { cbv [un_outbounds tight_bounds tight_upperbounds
-        prime_upperbound_list Partition.Partition.partition];
-        rewrite !map_length, seq_length; trivial. }
   Qed.
 
   Lemma from_bytes_func_correct :
@@ -441,11 +429,11 @@ Section UnsaturatedSolinas.
       as Hcorrect.
 
     eapply Signature.from_bytes_correct with (res:=res from_bytes_op);
-      handle_side_conditions; [ | ].
+      handle_side_conditions; [ loosen_bounds | bounds_length | | ].
     { (* output *value* is correct *)
       intros. specialize_correctness_hyp Hcorrect.
-      destruct Hcorrect. simpl_map_unsigned.
-      FtoZ. congruence. }
+      destruct Hcorrect. cbv [feval_alt].
+      FtoZ. simpl_map_unsigned. congruence. }
     { (* output *bounds* are correct *)
       intros. apply Hcorrect; auto. }
   Qed.
@@ -461,10 +449,16 @@ Section UnsaturatedSolinas.
       as Hcorrect.
 
     eapply Signature.to_bytes_correct with (res:=res to_bytes_op);
-      handle_side_conditions; [ | ].
+      handle_side_conditions; [ | | | ].
+    {
+      intros. eapply relax_list_Z_bounded_by; [| eauto]. apply byte_bounds_tighter_than.
+    }
+    {
+      intros. erewrite length_list_Z_bounded_by; [| eauto]. apply length_byte_bounds.
+    }
     { (* output *value* is correct *)
       intros. specialize_correctness_hyp Hcorrect.
-      rewrite Hcorrect.
+      rewrite Hcorrect. cbv [feval_alt Representation.eval_words_alt].
       rewrite F.to_Z_of_Z, <-M_eq.
       reflexivity. }
     { (* output *bounds* are correct *)
@@ -503,6 +497,9 @@ Definition field_parameters_prefixed
     (prefix ++ "to_bytes")
     (prefix ++ "copy")
     (prefix ++ "small_literal")
+    (prefix ++ "to_mont")
+    (prefix ++ "from_mont")
+    (prefix ++ "select_znz")
 .
 
 Local Ltac begin_derive_bedrock2_func :=
